theories/Environment/OverlayMap.v
@@ -1,0 +1,285 @@
+From Coq Require Import Lia Morphisms.
+From DeBrLevel Require Import LevelInterface Level MapLevelInterface MapLevel MapExtInterface 
+               MapExt.
+
+(** * Environment - Overlay - Map *)
+
+(** ** Module - Overlay *)
+Module OverlayMap (Data : IsLvlETWL) <: IsLvlET.
+
+(** *** Definition *)
+
+Include MapLvlD.MakeLvlMapLVLD Data.
+Import Raw Ext.
+
+(** **** ForAll property
+
+  MMaps does not provide a function that check if all elements in the environment satisfy a property [P]. Consequently we define it.
+*)
+Definition For_all (P : Lvl.t -> Data.t -> Prop) (o : t) := 
+  forall k d, find k o = Some d -> P k d.
+
+
+(** *** Property *)
+
+(** **** [For_all] property *)
+Section For_all.
+
+Hypothesis P : Lvl.t -> Data.t -> Prop. 
+
+#[export] Instance For_all_proper : Proper (eq ==> iff) (For_all P).
+Proof.
+  intros o o' Heqo; unfold For_all; split; intros HFa k d Hfi.
+  - rewrite <- Heqo in Hfi; auto.
+  - rewrite Heqo in Hfi; auto.
+Qed.
+
+Lemma For_all_empty_spec : For_all P empty.
+Proof. intros k d Hfi; inversion Hfi. Qed.
+
+Lemma For_all_Empty_spec (o : t) :
+  Empty o -> For_all P o.
+Proof.
+  intros HEmp k d Hfi; apply Empty_eq_spec in HEmp.
+  rewrite HEmp in Hfi; inversion Hfi.
+Qed.
+
+Lemma For_all_add_spec (k : Lvl.t) (d : Data.t) (o : t) :
+ P k d /\ For_all P o -> For_all P (add k d o).
+Proof.
+  intros [HP HFa] k' d' Hfi.
+  destruct (Lvl.eq_dec k' k) as [Heq | Hneq]; subst.
+  - rewrite add_eq_o in Hfi; auto.
+    inversion Hfi; now subst.
+  - rewrite add_neq_o in Hfi; auto.
+Qed.
+
+Lemma For_all_add_notin_spec (k : Lvl.t) (d : Data.t) (o : t) :
+ ~ In k o ->
+ ((P k d /\ For_all P o) <-> For_all P (add k d o)).
+Proof.
+  intro HnIn; split.
+  - apply For_all_add_spec.
+  - intro HFa; split.
+    -- apply HFa.
+       now rewrite add_eq_o.
+    -- intros k' d' Hfi. 
+       destruct (Lvl.eq_dec k' k) as [Heq | Hneq]; subst.
+       + exfalso; apply HnIn.
+         exists d'; now apply find_2.
+       + apply HFa.
+         now rewrite add_neq_o.
+Qed.
+
+End For_all.
+
+(** **** [valid] property *)
+
+Lemma valid_update_spec (m k : Lvl.t) (d : Data.t) (o : t) :
+  In k o -> valid m o -> Data.valid m d -> valid m (add k d o).
+Proof.
+  revert k d; induction o using map_induction; intros k d HIn Hvo Hvd.
+  - apply Empty_eq_spec in H; rewrite H in *.
+    inversion HIn; inversion H0.
+  - unfold Add in H0; rewrite H0 in *; clear H0.
+    apply valid_add_notin_spec in Hvo as [Hvx [Hve Hvo1]]; auto.
+    apply add_in_iff in HIn as [Heq | HIn]; subst.
+    -- rewrite add_shadow.
+       rewrite valid_add_notin_spec; auto.
+    -- destruct (Lvl.eq_dec k x) as [| Hneq]; subst; try contradiction.
+       rewrite add_add_2; auto.
+       eapply IHo1 in Hvo1; eauto.
+       rewrite valid_add_notin_spec; auto.
+       rewrite add_in_iff; intros [Hc | Hc]; subst; contradiction.
+Qed.
+
+Lemma valid_in_iff (m n k : Lvl.t) (d : Data.t) (o : t) :
+  valid m o -> In k (shift m n o) <-> In k o.
+Proof.
+  revert k; induction o using map_induction; intros k Hvo; split; intro HIn.
+  - rewrite shift_Empty_spec in HIn; auto.
+  - rewrite shift_Empty_spec; auto.
+  - unfold Add in *; rewrite H0 in *; clear H0. 
+    apply valid_add_notin_spec in Hvo as [Hvk [Hvd Hv]]; auto.
+    rewrite shift_add_notin_spec in HIn; auto.
+    rewrite add_in_iff in *; destruct HIn as [Heq | HIn]; subst.
+    -- left; rewrite Level.shift_valid_refl; auto.
+    -- right. rewrite <- IHo1; eauto.
+  - unfold Add in *; rewrite H0 in *; clear H0. 
+    apply valid_add_notin_spec in Hvo as [Hvk [Hvd Hv]]; auto.
+    rewrite shift_add_notin_spec; auto.
+    rewrite add_in_iff in *; destruct HIn as [Heq | HIn]; subst.
+    -- left; rewrite Level.shift_valid_refl; auto.
+    -- right. rewrite IHo1; eauto.
+Qed.
+
+(** **** [shift] property *)
+
+Lemma shift_new_in_spec (k : Lvl.t) (o : t) :
+  In k o ->  k < new_key o.
+Proof.
+  revert k; induction o using map_induction; intros k HIn.
+  - exfalso; destruct HIn as [d HM]; now apply (H k d).
+  - unfold Add in H0; rewrite H0 in *; clear H0.
+    apply add_in_iff in HIn as [Heq | HIn]; subst.
+    -- destruct (Lvl.leb_spec (new_key o1) (S k)).
+       + rewrite new_key_add_ge_spec; auto; lia.
+       + rewrite new_key_add_lt_spec; auto; lia.
+    -- apply IHo1 in HIn as Hnew.
+       destruct (Lvl.leb_spec (new_key o1) (S x)).
+       + rewrite new_key_add_ge_spec; auto; lia.
+       + rewrite new_key_add_lt_spec; auto; lia.
+Qed.
+
+Lemma shift_gt_iff (m n x y : Lvl.t) :
+  x > y <-> (Level.shift m n x) > (Level.shift m n y).
+Proof.
+  unfold Level.shift; split; intro Hgt;
+  destruct (Level.leb_spec m x); destruct (Level.leb_spec m y); lia.
+Qed.
+
+Lemma shift_le_spec (m n x : Lvl.t) :
+  x <= (Level.shift m n x).
+Proof.
+  unfold Level.shift; destruct (Level.leb_spec m x); lia.
+Qed.
+
+Lemma shift_max_key_gt_iff (m n x : Lvl.t) (o : t) :
+  max_key o > x <-> max_key (shift m n o) > (Level.shift m n x).
+Proof.
+  revert x; induction o using map_induction; intro y.
+  - split; intro Hmax.
+    -- rewrite max_key_Empty_spec in Hmax; auto; lia.
+    -- rewrite shift_Empty_spec in Hmax; auto.
+       rewrite max_key_Empty_spec in Hmax; auto; lia.
+  - split; intro Hmax;
+    unfold Add in H0; rewrite H0 in *; clear H0.
+    -- destruct (Level.leb_spec (max_key o1) x) as [Hle | Hgt].
+       + rewrite max_key_add_ge_spec in Hmax; auto; try lia.
+         rewrite shift_add_spec.
+         rewrite (shift_in_iff m n) in H.
+         destruct (Level.leb_spec (max_key (shift m n o1)) (Level.shift m n x)) as [Hle' | Hgt'].
+         ++ rewrite max_key_add_ge_spec; auto; try lia.
+            now apply shift_gt_iff.
+         ++ rewrite max_key_add_lt_spec; auto; try lia.
+            assert (max_key o1 > x) by (rewrite IHo1; lia); lia.
+       + rewrite max_key_add_lt_spec in Hmax; auto; try lia.
+         rewrite shift_add_spec.
+         rewrite (shift_in_iff m n) in H.
+         destruct (Level.leb_spec (max_key (shift m n o1)) (Level.shift m n x)) as [Hle' | Hgt'].
+         ++ rewrite IHo1 in Hmax.
+            rewrite max_key_add_ge_spec; auto; lia.
+         ++ rewrite max_key_add_lt_spec; auto; try lia.
+            now rewrite <- IHo1.
+    -- rewrite shift_add_spec in Hmax.
+       rewrite (shift_in_iff m n) in H.
+       destruct (Level.leb_spec (max_key (shift m n o1)) (Level.shift m n x)) as [Hle | Hgt].
+       + rewrite max_key_add_ge_spec in Hmax; auto; try lia.
+         rewrite <- (shift_in_iff m n) in H.
+         destruct (Level.leb_spec (max_key o1) x) as [Hle' | Hgt'].
+         ++ rewrite max_key_add_ge_spec; auto; try lia.
+            now apply shift_gt_iff in Hmax.
+         ++ rewrite max_key_add_lt_spec; auto; try lia.
+            rewrite <- shift_gt_iff in Hmax; lia.
+       + rewrite max_key_add_lt_spec in Hmax; auto; try lia.
+         rewrite <- (shift_in_iff m n) in H.
+         destruct (Level.leb_spec (max_key o1) x) as [Hle' | Hgt'].
+         ++ rewrite max_key_add_ge_spec; auto; try lia.
+            rewrite <- IHo1 in Hmax; lia.
+         ++ rewrite max_key_add_lt_spec; auto; try lia.
+            rewrite <- IHo1 in Hmax; lia.
+Qed. 
+
+Lemma shift_max_key_le_spec (m n : Lvl.t) (o : t) :
+  max_key o <= max_key (shift m n o).
+Proof.
+  induction o using map_induction.
+  - now rewrite shift_Empty_spec.
+  - unfold Add in H0; rewrite H0; clear H0. 
+    rewrite shift_add_spec.
+    destruct (Level.leb_spec (max_key o1) x) as [Hle | Hgt].
+    -- rewrite max_key_add_ge_spec; auto; try lia.
+       rewrite (shift_in_iff m n) in H.
+       destruct (Level.leb_spec (max_key (shift m n o1)) (Level.shift m n x)) as [Hle' | Hgt'].
+       + rewrite max_key_add_ge_spec; auto; try lia.
+         apply shift_le_spec.
+       + rewrite max_key_add_lt_spec; auto; try lia.
+         assert (Hgt : max_key (shift m n o1) > Level.shift m n x) by lia.
+         rewrite <- shift_max_key_gt_iff in Hgt; lia.
+    -- rewrite max_key_add_lt_spec; auto; try lia.
+       rewrite (shift_in_iff m n) in H.
+       destruct (Level.leb_spec (max_key (shift m n o1)) (Level.shift m n x)) as [Hle' | Hgt'].
+       + rewrite max_key_add_ge_spec; auto; lia.
+       + rewrite max_key_add_lt_spec; auto; lia.
+Qed.
+       
+Lemma shift_new_key_le_spec (m n : Lvl.t) (o : t) :
+  new_key o <= new_key (shift m n o).
+Proof.
+  unfold new_key; destruct (is_empty o) eqn:Hemp; try lia.
+  destruct (is_empty (shift m n o)) eqn:Hemp'.
+  - apply is_empty_2 in Hemp'. 
+    rewrite <- (shift_Empty_iff m n) in Hemp'.
+    apply is_empty_1 in Hemp'.
+    rewrite Hemp in Hemp'; now inversion Hemp'.
+  - assert (max_key o <= max_key (shift m n o)); try lia.
+    apply shift_max_key_le_spec.
+Qed.
+
+Lemma shift_in_e_spec (m n k : Lvl.t) (o : t) :
+  In k (shift m n o) -> exists (k' : Lvl.t), k = Level.shift m n k'.
+Proof.
+  revert k; induction o using map_induction; intros k HIn.
+  - rewrite shift_Empty_spec in HIn; auto.
+    exfalso; destruct HIn as [v HM]; now apply (H k v).
+  - unfold Add in H0; rewrite H0 in *; clear H0.
+    rewrite shift_add_spec in HIn.
+    apply add_in_iff in HIn as [Heq | Hneq]; auto.
+    now exists x.
+Qed.
+
+(* Lemma shift_find_spec_3 : forall lb k r V V',
+  (lb ⊩ r)%r -> In r V ->
+  find r V = find r V' -> find r (shift lb k V) = find r (shift lb k V').
+Proof.
+  intros. destruct H0 as [v HfV]; apply find_1 in HfV.
+  apply shift_find_iff with (lb := lb) (k := k) in HfV as HfV1.
+  rewrite H1 in HfV. 
+  apply shift_find_iff with (lb := lb) (k := k) in HfV as HfV2.
+  rewrite Resource.shift_valid_refl in *; auto. now rewrite HfV1, HfV2. 
+Qed. *)
+
+Lemma shift_find_e_spec_1 (m n k : Lvl.t) (d : Data.t) (o : t) :
+  find k (shift m n o) = Some d -> 
+  (exists k', k = Level.shift m n k') /\ (exists d', (Data.eq d (Data.shift m n d'))).
+Proof.
+  intro Hfi.
+  assert (HIn : In k (shift m n o)). { now exists d; apply find_2. }
+  apply shift_in_e_spec in HIn; split; auto.
+  destruct HIn as [k' Heq]; subst.
+  now apply shift_find_e_spec in Hfi.
+Qed.
+
+End OverlayMap.
+
+
+Module OverlayMapBdl (Data : IsBdlLvlETWL) <: IsBdlLvlET.
+
+Include OverlayMap Data.
+
+Lemma shift_valid_refl (lb k : Lvl.t) (t : t) : valid lb t -> eq (shift lb k t) t.
+Proof.
+  induction t using map_induction; intro Hvt.
+  - now apply shift_Empty_spec.
+  - unfold Add in H0; rewrite H0 in *; clear H0.
+    apply valid_add_notin_spec in Hvt as [Hvx [Hve Hvt]]; auto. 
+    rewrite shift_add_spec.
+    rewrite IHt1; auto.
+    rewrite Level.shift_valid_refl; auto.
+
+    replace (Data.shift lb k e) with e; try reflexivity.
+    apply Data.eq_leibniz.
+    now rewrite Data.shift_valid_refl; auto.
+Qed.
+
+End OverlayMapBdl.
