theories/Environment/RContext.v
@@ -1,5 +1,5 @@
 From Coq Require Import Lia Classes.Morphisms.
-From Mecha Require Import Typ Resource.
+From Mecha Require Import Typ Resource OverlayMap.
 From DeBrLevel Require Import LevelInterface Level MapLevelInterface MapLevel.
 Import ResourceNotations TypNotations.
 
@@ -13,135 +13,30 @@ Module RContext <: IsBdlLvlET.
 
 (** *** Definition *)
 
-Include MapLvlD.MakeBdlLvlMapLVLD PairTyp.
+Include OverlayMapBdl PairTyp.
 Import Raw Ext.
 
 Open Scope ptyp_scope.
 
 (** *** Property *)
 
-(** **** [shift] extra property *)
-
-Lemma shift_max_key_gt (m n x : lvl) (c : t) :
-  max_key c > x <-> max_key (shift m n c) > ([⧐m – n] x)%r.
-Proof.
-  revert x; induction c using map_induction; intro y.
-  - split; intros.
-    -- rewrite max_key_Empty_spec in H0; auto. lia.
-    -- rewrite shift_Empty_spec in H0; auto.
-       rewrite max_key_Empty_spec in H0; auto. lia.
-  - split; intros.
-    -- unfold Add in *; rewrite H0 in *; clear H0.
-       apply (max_key_add_spec) with (v := e) in H as H'.
-       destruct H' as [[Heq Hle] | [Heq Hgt]].
-       + rewrite Heq in *; clear Heq.
-         rewrite (shift_in_iff m n) in H.
-         apply (max_key_add_spec) with (v := <[ [⧐m – n] e ]>) in H as H''.
-         destruct H'' as [[Heq Hle'] | [Heq Hgt']].
-         ++ rewrite shift_add_spec. 
-            rewrite Heq.
-            unfold Level.shift.
-            destruct (Level.leb_spec m x); destruct (Level.leb_spec m y); lia.
-         ++ rewrite <- IHc1 in Hgt'. lia.
-       + rewrite IHc1 in Hgt.
-         rewrite shift_add_spec.
-         rewrite max_key_add_lt_spec; auto.
-         ++ now rewrite <- IHc1; rewrite <- Heq.
-         ++ now rewrite <- shift_in_iff.
-    -- unfold Add in *; rewrite H0 in *; clear H0.
-       rewrite shift_add_spec in *.
-       apply (max_key_add_spec) with (v := e) in H as H'.
-       destruct H' as [[Heq Hle] | [Heq Hgt]].
-       + rewrite Heq in *; clear Heq.
-         rewrite (shift_in_iff m n) in H.
-         apply (max_key_add_spec) with (v := <[ [⧐m – n] e ]>) in H as H''.
-         destruct H'' as [[Heq Hle'] | [Heq Hgt']].
-         ++ rewrite Heq in *.
-            unfold Level.shift in *.
-            destruct (Level.leb_spec m x); destruct (Level.leb_spec m y); lia.
-         ++ rewrite <- IHc1 in Hgt'. lia.
-       + rewrite IHc1 in Hgt.
-         rewrite max_key_add_lt_spec in H1; auto.
-         ++ now rewrite Heq; rewrite IHc1.
-         ++ now rewrite <- shift_in_iff.
-Qed. 
-
-Lemma shift_max_key_le (m n : Lvl.t) (c1 : t) :
-  max_key c1 <= max_key (shift m n c1).
-Proof.
-  induction c1 using map_induction.
-  - now rewrite shift_Empty_spec.
-  - unfold Add in H0; rewrite H0; clear H0. 
-    rewrite shift_add_spec.
-    apply (max_key_add_spec) with (v := e) in H as H'.
-    rewrite (shift_in_iff m n) in H.
-    apply (max_key_add_spec) with (v := <[ [⧐m – n] e ]>) in H as H''.
-    destruct H' as [[Heq Hle] | [Heq Hgt]].
-    -- rewrite Heq; clear Heq.
-       destruct H'' as [[Heq Hle'] | [Heq Hgt']].
-       + rewrite Heq; clear Heq.
-         unfold Level.shift; destruct (Level.leb m x); lia.
-       + rewrite Heq; clear Heq. 
-         rewrite <- shift_max_key_gt in Hgt'.
-         lia.
-    -- rewrite Heq; clear Heq.
-       destruct H'' as [[Heq Hle'] | [Heq Hgt']].
-       + rewrite Heq; clear Heq. lia.
-       + now rewrite Heq; clear Heq.
-Qed.
-       
-Lemma shift_new_key_le (m n : Lvl.t) (c1 : t) :
-  new_key c1 <= new_key (shift m n c1).
-Proof.
-  unfold new_key; destruct (is_empty c1) eqn:Hemp.
-  - lia.
-  - destruct (is_empty (shift m n c1)) eqn:Hemp'.
-    -- apply is_empty_2 in Hemp'. 
-       rewrite <- (shift_Empty_iff m n) in Hemp'.
-       apply is_empty_1 in Hemp'.
-       rewrite Hemp in Hemp'; now inversion Hemp'.
-    -- assert (max_key c1 <= max_key (shift m n c1)).
-       + apply shift_max_key_le.
-       + lia.
-Qed.
-
-
 (** **** Wormholes specification *)
 
-Lemma max_key_wh_spec : forall (m : t) (v v' : πΤ),
-  max_key (add (S (S (max_key m))) v (add (S (max_key m)) v' m)) = S (S (max_key m)).
-Proof.
-  intros m v v'.
-  apply max_key_add_ge_spec.
-  - apply max_key_notin_spec. 
-    rewrite max_key_add_ge_spec; auto.
-    apply max_key_notin_spec; auto.
-  - rewrite max_key_add_ge_spec; auto.
-    apply max_key_notin_spec; auto.
-Qed.
-
-Lemma new_key_wh_spec : forall (m : t) (v v' : πΤ),
+Lemma new_key_wh_spec (m : t) (v v' : πΤ) :
   new_key (add (S (new_key m)) v (add (new_key m) v' m)) = S (S (new_key m)).
 Proof.
-  intros m v v'; unfold new_key; 
-  rewrite is_empty_add_spec; destruct (is_empty m) eqn:Heq.
-  - rewrite max_key_add_ge_spec; auto.
-    -- apply is_empty_iff in Heq; unfold Empty,not in *; 
-      intros. destruct H. apply (Heq 1 x). apply add_mapsto_iff in H.
-      destruct H; destruct H; try lia; assumption.
-    -- rewrite max_key_add_ge_spec; auto.
-      + apply is_empty_iff in Heq. unfold Empty,not in *; 
-        intros; destruct H; now apply (Heq 0 x).
-      + rewrite max_key_Empty_spec; auto. now apply is_empty_iff.
-  - f_equal. apply max_key_wh_spec.
+  repeat rewrite new_key_add_ge_spec; auto.
+  - apply new_key_notin_spec; 
+    rewrite new_key_add_ge_spec; auto.
+    apply new_key_notin_spec; auto.
+  - apply new_key_notin_spec; auto.
 Qed.
 
-Lemma valid_wh_spec : forall (m : t) (v v' : πΤ),
-  valid (new_key m) m -> 
-  (new_key m) ⊩ v -> (new_key m) ⊩ v' -> 
+Lemma valid_wh_spec (m : t) (v v' : πΤ) :
+  valid (new_key m) m -> (new_key m) ⊩ v -> (new_key m) ⊩ v' -> 
   valid (S (S (new_key m))) (add (S (new_key m)) v (add (new_key m) v' m)).
 Proof.
-  intros m v v' Hvm Hvv Hvv'. 
+  intros Hvm Hvv Hvv'. 
   apply valid_add_notin_spec.
   - rewrite add_in_iff; intro Ha. 
     destruct Ha as [Heq | HIn]; try lia.
@@ -165,12 +60,13 @@ Qed.
 Proof. intros x y Heqx c c' Heqc; subst; now rewrite Heqc. Qed.
 
 #[export] Instance find_rctx : Proper (Logic.eq ==> eq ==> Logic.eq) find.
-Proof. repeat red; intros; subst. now rewrite H0. Qed.
+Proof. intros x y Heqx c c' Heqc; subst; now rewrite Heqc. Qed.
 
 #[export] Instance Empty_rctx : Proper (eq ==> iff) Empty.
 Proof. intros c c' Heq; now rewrite Heq. Qed.
 
-#[export] Instance Add_rctx : Proper (Resource.eq ==> PairTyp.eq ==> eq ==> eq ==> iff) (@Add PairTyp.t).
+#[export] Instance Add_rctx : 
+  Proper (Resource.eq ==> PairTyp.eq ==> eq ==> eq ==> iff) (@Add PairTyp.t).
 Proof. 
   intros x x' HeqV ty ty' HeqT c c' Heq c1 c1' Heq1.
   apply PairTyp.eq_leibniz in HeqT; subst.
