theories/Environment/REnvironment.v
@@ -1,0 +1,387 @@
+From Coq Require Import Lia Arith.PeanoNat Classical_Prop Morphisms SetoidList.
+From Mecha Require Import OverlayMap Resource Resources Term Cell.
+From Mecha Require Evaluation_Transition.
+From DeBrLevel Require Import LevelInterface MapLevelInterface MapLevel MapExtInterface MapExt.
+Import ResourceNotations TermNotations CellNotations 
+       ResourcesNotations SetNotations.
+
+
+
+(** * Environment - Resource Environment
+
+  The functional transition, defined in [Functional_Transition.v], requires a local memory represented by an environment. We defined here the resource environment which maps resource names with memory cells, defined in [Cell.v]. This environment is an interface between the program and the outside.
+*)
+
+(** ** Module - Resource Environment *)
+Module REnvironment <: IsLvlET.
+
+(** *** Definition *)
+Include OverlayMap Cell.
+Import Raw Ext.
+
+Open Scope cell_scope.
+Open Scope term_scope.
+
+Module ET := Evaluation_Transition.
+Module RS := Resources.St.
+
+(** **** Initialize an environment
+
+  For each instant, local resource names that represent a writing interaction have their memory cells initialized as unused with a [unit] term. This function takes a resource set [rs] and an environement [V] and produces an environment where all resource names in [rs] are initialized.
+*)
+Definition init_write_func (r : resource) (V : t) : t := add r (⩽ unit … ⩾) V.
+
+Definition init_write (rs : resources) (V : t) := RS.fold (init_write_func) rs V.
+
+(** **** Halts 
+
+  In the functional transition proofs, we assume that all elements in the input resource environment halts. Thus, we define this property here with [For_all].
+  An environment has the halting property if and only if each term in it halts. 
+*)
+Definition halts (k : lvl) := For_all (fun _ d => ET.halts k (Cell.extract d)).
+
+(** *** To be used or not to be *)
+
+Definition   used r (V : t) : Prop := Cell.opt_used (find r V). 
+Definition unused r (V : t) : Prop := Cell.opt_unused (find r V).
+
+(** *** Property *)
+
+(** **** [unused]-[used] property *)
+
+#[export] Instance unused_proper : Proper (Logic.eq ==> eq ==> iff) unused.
+Proof.
+  intros r' r Heqr V V' HeqV; subst; unfold unused,Cell.opt_unused.
+  now rewrite HeqV.
+Qed.
+
+Lemma unused_Empty_spec (r : resource) (V : t) :
+  Empty V -> ~ (unused r V).
+Proof.
+  unfold unused, Cell.opt_unused; intros Hemp Husd.
+  assert (HnIn : ~ In r V).
+  - intros [v HM]; now apply (Hemp r v).
+  - apply not_in_find in HnIn.
+    rewrite HnIn in Husd; contradiction. 
+Qed.
+
+Lemma unused_add_spec (r r' : resource) (v : 𝑣) (V : t) :
+  (unused r (add r' v V)) -> (Cell.unused v) \/ (unused r V).
+Proof.
+  unfold unused, Cell.opt_unused; intro Husd; 
+  destruct (Resource.eq_dec r r') as [Heq | Hneq]; subst.
+  - rewrite add_eq_o in Husd; auto.
+  - rewrite add_neq_o in Husd; auto.
+Qed.
+
+Lemma unused_add_spec_1 (r r' : resource) (v : 𝑣) (V : t) :
+  (Cell.unused v) /\ (unused r V) -> (unused r (add r' v V)).
+Proof.
+  unfold unused, Cell.opt_unused; intros [HCusd Husd].
+  destruct (Resource.eq_dec r r') as [Heq | Hneq]; subst.
+  - rewrite add_eq_o; auto.
+  - rewrite add_neq_o; auto.
+Qed.
+
+Lemma unused_add_eq_spec (r : resource) (v : 𝑣) (V : t) :
+  (Cell.unused v) -> (unused r (add r v V)).
+Proof. unfold unused, Cell.opt_unused; intro Husd; rewrite add_eq_o; auto. Qed.
+
+Lemma unused_add_neq_spec (r r' : resource) (v : 𝑣) (V : t) :
+  r <> r' -> (unused r V) -> (unused r (add r' v V)).
+Proof. unfold unused, Cell.opt_unused; intro Husd; rewrite add_neq_o; auto. Qed.
+
+#[export] Instance used_proper : Proper (Logic.eq ==> eq ==> iff) used.
+Proof.
+  intros r' r Heqr V V' HeqV; subst; unfold used,Cell.opt_used.
+  now rewrite HeqV.
+Qed.
+
+Lemma used_Empty_spec (r : resource) (V : t) :
+  Empty V -> ~ (used r V).
+Proof.
+  unfold used, Cell.opt_used; intros Hemp Husd.
+  assert (HnIn : ~ In r V).
+  - intros [v HM]; now apply (Hemp r v).
+  - apply not_in_find in HnIn.
+    rewrite HnIn in Husd; contradiction. 
+Qed.
+
+Lemma used_add_spec (r r' : resource) (v : 𝑣) (V : t) :
+  (used r (add r' v V)) -> (Cell.used v) \/ (used r V).
+Proof.
+  unfold used, Cell.opt_used; intro Husd; 
+  destruct (Resource.eq_dec r r') as [Heq | Hneq]; subst.
+  - rewrite add_eq_o in Husd; auto.
+  - rewrite add_neq_o in Husd; auto.
+Qed.
+
+Lemma used_add_spec_1 (r r' : resource) (v : 𝑣) (V : t) :
+  (Cell.used v) /\ (used r V) -> (used r (add r' v V)).
+Proof.
+  unfold used, Cell.opt_used; intros [HCusd Husd].
+  destruct (Resource.eq_dec r r') as [Heq | Hneq]; subst.
+  - rewrite add_eq_o; auto.
+  - rewrite add_neq_o; auto.
+Qed.
+
+Lemma used_add_eq_spec (r : resource) (v : 𝑣) (V : t) :
+  (Cell.used v) -> (used r (add r v V)).
+Proof. unfold used, Cell.opt_used; intro Husd; rewrite add_eq_o; auto. Qed.
+
+Lemma used_add_neq_spec (r r' : resource) (v : 𝑣) (V : t) :
+  r <> r' -> (used r V) -> (used r (add r' v V)).
+Proof. unfold used, Cell.opt_used; intro Husd; rewrite add_neq_o; auto. Qed.
+
+(** **** [init_write] property *)
+
+
+#[export] Instance init_write_func_proper : Proper (Logic.eq ==> eq ==> eq) init_write_func.
+Proof. 
+  unfold init_write_func; intros k' k Heqk V V' HeqV. 
+  subst; now rewrite HeqV. 
+Qed.
+
+Lemma init_write_func_transpose : transpose eq init_write_func.
+Proof. 
+  unfold init_write_func; intros k k' V. 
+  destruct (Resource.eq_dec k k') as [Heq | Hneq]; subst.
+  - reflexivity.
+  - now rewrite add_add_2; auto.
+Qed.
+
+#[local] Hint Resolve init_write_func_proper init_write_func_transpose : core.
+
+Lemma init_write_Empty_spec (rs : resources) (V : t) :
+  RS.Empty rs -> eq (init_write rs V) V.
+Proof.
+  intro Hemp; unfold init_write.
+  apply RS.empty_is_empty_1 in Hemp.
+  rewrite RS.fold_equal with (eqA := eq); eauto.
+  now rewrite RS.fold_empty.
+Qed.
+
+Lemma init_write_add_spec (r : resource) (rs : resources) (V : t) :
+  (r ∉ rs)%s ->
+  eq (init_write (RS.add r rs) V) (add r (⩽ unit … ⩾) (init_write rs V)). 
+Proof.
+  unfold init_write; intro HnIn.
+  now rewrite RS.fold_add with (eqA := eq); auto.
+Qed.
+
+Lemma init_write_unused (rs : resources) (V : t) (r : resource) :
+  (r ∈ rs)%s -> unused r (init_write rs V).
+Proof.
+  revert r; induction rs using RS.set_induction; intros r HIn.
+  - unfold RS.Empty in H. 
+    exfalso; now apply (H r).
+  - apply RS.Add_inv in H0; subst.
+    rewrite init_write_add_spec; auto.
+    apply RS.add_spec in HIn as [Heq | HIn]; subst. 
+    -- apply unused_add_eq_spec; now red.
+    -- assert (r <> x) by (intro; subst; contradiction).
+       apply unused_add_neq_spec; auto. 
+Qed.
+
+Lemma init_write_find_spec (rs : resources) (V : t) (r : resource) (v : 𝑣) :
+  find r (init_write rs V) = Some v -> (r ∈ rs)%s \/ find r V = Some v.
+Proof.
+  revert r v; induction rs using RS.set_induction; intros r v Hfi.
+  - rewrite init_write_Empty_spec in Hfi; auto.
+  - apply RS.Add_inv in H0; subst.
+    rewrite init_write_add_spec in Hfi; auto.
+    destruct (Resource.eq_dec x r) as [Heq | Hneq]; subst.
+    -- left; rewrite RS.add_spec; auto.
+    -- rewrite add_neq_o in Hfi; auto.
+       apply IHrs1 in Hfi as [HIn | Hfi]; auto.
+       left; rewrite RS.add_spec; auto.
+Qed.
+
+Lemma init_write_in_iff (rs : resources) (V : t) (r : resource) :
+  In r (init_write rs V) <-> (r ∈ rs)%s \/ In r V.
+Proof.
+  revert r; induction rs using RS.set_induction; intro r; split.
+  - intro HIn. rewrite init_write_Empty_spec in HIn; auto.
+  - intros [HIn | HIn].
+    -- exfalso. now apply (H r).
+    -- now rewrite init_write_Empty_spec.
+  - intro HIn; apply RS.Add_inv in H0; subst. 
+    rewrite init_write_add_spec in HIn; auto.
+    apply add_in_iff in HIn as [Heq | HIn]; subst.
+    -- left; rewrite RS.add_spec; auto.
+    -- apply IHrs1 in HIn as [HIn | HIn]; auto.
+       left; rewrite RS.add_spec; auto.
+  - intros [HIn | HIn]; apply RS.Add_inv in H0; subst.
+    -- rewrite init_write_add_spec; auto.
+       rewrite add_in_iff.
+       apply RS.add_spec in HIn as [Heq | HIn]; auto.
+       right; rewrite IHrs1; now left.
+    -- rewrite init_write_add_spec; auto.
+       rewrite add_in_iff; right.
+       rewrite IHrs1; now right. 
+Qed. 
+       
+(* Lemma init_write_Forall_unused : forall rs V,
+  For_all (fun _ v => Cell.unused v) V ->
+  For_all (fun _ v => Cell.unused v) (init_write rs V).
+Proof.
+  unfold For_all in *; intros.
+  apply init_write_find_spec in H0 as H0'; destruct H0'; auto.
+  - eapply init_write_unused in H1; eauto.
+    destruct H1; rewrite H0 in H1; inversion H1. now simpl.
+  - eapply H; eauto.
+Qed. *)
+
+
+(** *** [valid] property *)
+
+Lemma valid_wh_spec (v v' : 𝑣) (V : t) :
+  valid (new_key V) V -> ((new_key V) ⊩ v)%cl -> ((new_key V) ⊩ v')%cl -> 
+  valid (S (S (new_key V))) 
+        (add (S (new_key V)) v 
+        (add (new_key V) (Cell.shift (new_key V) 2 v') (shift (new_key V) 2 V))).
+Proof.
+  intros HvV Hvv Hvv'; do 2 try rewrite valid_add_notin_spec.
+  - repeat split; try (unfold Resource.valid; lia). 
+    -- apply Cell.valid_weakening with (k := new_key V); auto.
+    -- replace (S (S (new_key V))) with ((new_key V) + 2) by lia. 
+       now apply Cell.shift_preserves_valid_1.
+    -- replace (S (S (new_key V))) with ((new_key V) + 2) by lia. 
+       now apply shift_preserves_valid_1.  
+  - apply new_key_notin_spec; auto; rewrite shift_new_spec; auto.
+  - apply new_key_notin_spec; rewrite new_key_add_ge_spec; auto.
+    -- apply new_key_notin_spec; auto; rewrite shift_new_spec; auto.
+    -- rewrite shift_new_spec; auto.
+Qed.
+
+(** *** [halts] property *)
+
+Lemma halts_add_spec (k : lvl) (r : resource) (v : 𝑣) (V : t) :
+  (ET.halts k (Cell.extract v)) /\ halts k V -> halts k (add r v V).
+Proof.
+  intros [Hltv Hltm] r' v' Hfi.
+  destruct (Resource.eq_dec r r') as [| Hneq]; subst.
+  - rewrite add_eq_o in Hfi; auto.
+    inversion Hfi; subst; auto.
+  - rewrite add_neq_o in Hfi; auto.
+    now apply Hltm in Hfi.
+Qed.
+
+Lemma halts_init_write (k : lvl) (rs : resources) (V : t) :
+  halts k V -> halts k (init_write rs V).
+Proof.
+  induction rs using Resources.St.set_induction; intro Hlt.
+  - now rewrite init_write_Empty_spec.
+  - apply RS.Add_inv in H0; subst.
+    rewrite init_write_add_spec; auto.
+    apply halts_add_spec; split; auto.
+    red; exists <[unit]>; split.
+    -- apply ET.multi_unit.
+    -- now constructor.
+Qed.
+
+Lemma halts_weakening (m n : lvl) (V : t) : 
+  m <= n -> halts m V -> halts n (shift m (n - m) V).
+Proof.
+  intros Hle Hlt r v Hfi. 
+  apply shift_find_e_spec_1 in Hfi as HI.
+  destruct HI as [[r' Heqr'] [v' Heqv']]; subst.
+  rewrite <- shift_find_iff in Hfi. 
+  destruct v'; simpl in *; 
+  apply ET.halts_weakening; auto; apply Hlt in Hfi; now simpl in *.
+Qed.
+
+Lemma halts_weakening_1 (m n : lvl) (V : t) : 
+  halts m V -> halts (m + n) (shift m n V).
+Proof.
+  intro Hlt; replace n with ((m + n) - m) at 2 by lia.
+  apply halts_weakening; auto; lia.
+Qed.
+
+(** *** [new_key] property *)
+
+Lemma new_key_wh_spec (v v' : 𝑣) (V : t) :
+  new_key (add (S (new_key V)) v 
+          (add (new_key V) (Cell.shift (new_key V) 2 v') 
+                           (shift (new_key V) 2 V))) = S (S (new_key V)).
+Proof.
+  repeat rewrite new_key_add_ge_spec; auto.
+  - apply new_key_notin_spec; rewrite new_key_add_ge_spec; auto.
+    -- apply new_key_notin_spec; rewrite shift_new_spec; auto.
+    -- rewrite shift_new_spec; auto.
+  - apply new_key_notin_spec; rewrite shift_new_spec; auto.
+  - rewrite shift_new_spec; auto.
+Qed.
+
+
+(** *** Morphism *)
+
+#[export] Instance in_renv : Proper (Logic.eq ==> eq ==> iff) In.
+Proof. intros k' k Heqk V V' HeqV; subst; now rewrite HeqV. Qed.
+
+#[export] Instance Add_renv : 
+  Proper (Resource.eq ==> Cell.eq ==> eq ==> eq ==> iff) (@Add Cell.t).
+Proof.
+  intros k' k Heqk d d' Heqd V V' HeqV V1 V1' HeqV1; unfold Add.
+  now rewrite Heqk, Heqd, HeqV, HeqV1. 
+Qed.
+
+#[export] Instance halts_renv : Proper (Logic.eq ==> eq ==> iff) halts. 
+Proof. unfold halts; intros m n Heqm V V' HeqV; subst; now rewrite HeqV. Qed.
+
+End REnvironment.
+
+(** ---- *)
+
+(** ** Notation - Resource Environment *)
+
+Module REnvironmentNotations.
+
+(** *** Scope *)
+Declare Scope renvironment_scope.
+Delimit Scope renvironment_scope with re.
+
+(** *** Notation *)
+Definition 𝐕 := REnvironment.t.
+
+Notation "∅" := REnvironment.Raw.empty (at level 0, no associativity) : renvironment_scope. 
+Notation "V '⁺'" := (REnvironment.Ext.new_key V) (at level 16) : renvironment_scope.
+Notation "r '∉' Re" := (~ (REnvironment.Raw.In r Re)) 
+                       (at level 75, no associativity) : renvironment_scope. 
+Notation "'isEmpty(' Re ')'" := (REnvironment.Empty Re) (at level 20, no associativity) : renvironment_scope. 
+Notation "'Add'" := (REnvironment.Add) (at level 20, no associativity) : renvironment_scope. 
+Notation "R '⌊' x '⌋'"  := (REnvironment.Raw.find x R) (at level 15, x constr) : renvironment_scope.
+Notation "'max(' R ')'"  := (REnvironment.Ext.max_key R) (at level 15) : renvironment_scope.
+Notation "⌈ x ⤆ v '⌉' R"  := (REnvironment.Raw.add x v R) 
+                              (at level 15, x constr, v constr) : renvironment_scope.
+Notation "'[⧐' lb '–' k ']' t" := (REnvironment.shift lb k t) 
+                                   (at level 65, right associativity) : renvironment_scope.
+
+Infix "⊆" := REnvironment.Submap (at level 60, no associativity) : renvironment_scope. 
+Infix "∈" := REnvironment.Raw.In (at level 60, no associativity) : renvironment_scope. 
+Infix "=" := REnvironment.eq : renvironment_scope.
+Infix "⊩" := REnvironment.valid (at level 20, no associativity) : renvironment_scope.
+
+(** *** Morphism *)
+
+Import REnvironment.
+
+#[export] Instance equiv_renv : Equivalence REnvironment.eq := _.
+#[export] Instance max_renv : Proper (eq ==> Logic.eq) (Ext.max_key) := Ext.max_key_eq.
+#[export] Instance new_renv : Proper (eq ==> Logic.eq) (Ext.new_key) := Ext.new_key_eq. 
+#[export] Instance in_renv :  Proper (Logic.eq ==> eq ==> iff) (Raw.In) := _.
+#[export] Instance find_renv : Proper (Logic.eq ==> eq ==> Logic.eq) (Raw.find) := _.
+#[export] Instance Empty_renv : Proper (eq ==> iff) (Empty) := _.
+#[export] Instance Add_renv : 
+  Proper (Resource.eq ==> Cell.eq ==> eq ==> eq ==> iff) (@REnvironment.Add Cell.t) := _.
+#[export] Instance add_renv : 
+  Proper (Resource.eq ==> Cell.eq ==> REnvironment.eq ==> REnvironment.eq) (@Raw.add Cell.t) := _.
+#[export] Instance Submap_env : Proper (eq ==> eq ==> iff) Submap := _.
+#[export] Instance Submap_env_po : PreOrder Submap := Submap_po.
+#[export] Instance valid_renv : Proper (Logic.eq ==> eq ==> iff) valid := _.
+#[export] Instance shift_renv : Proper (Logic.eq ==> Logic.eq ==> eq ==> eq) shift := _.
+#[export] Instance halts_renv : Proper (Logic.eq ==> eq ==> iff) halts := _. 
+#[export] Instance unused_renv : Proper (Logic.eq ==> eq ==> iff) unused := _.
+#[export] Instance used_renv : Proper (Logic.eq ==> eq ==> iff) used := _.
+
+End REnvironmentNotations.
