theories/Environment/ReadStock.v
@@ -1,0 +1,307 @@
+From Coq Require Import Lia Arith.PeanoNat Morphisms.
+From Mecha Require Import Resource Resources Term REnvironment Cell OverlayMap.
+From DeBrLevel Require Import LevelInterface MapLevelInterface MapLevel MapExtInterface MapExt.
+Import ResourceNotations TermNotations REnvironmentNotations CellNotations
+       ResourcesNotations SetNotations.
+
+
+(** * Environment - Virtual Resource Environment - Reader
+
+  In the functional transition there are two kind of environment: the resource environment and the stock. The former, defined in [REnvironment.v], represents the local memory during an instant. The latter, defined in [Stock.v], keeps local resource names with their initial value. [ReadStock] is a part of the stock. It maps resource names with terms, i.e, it binds local resource names, used for a reading interaction, with their initial value.
+*)
+
+(** ** Module - Virtual Resource Environment - Reader *)
+Module ReadStock <: IsLvlET.
+
+Include OverlayMap Term.
+Import Raw Ext.
+
+Module ET := Evaluation_Transition.
+Module RE := REnvironment.
+
+(** *** Definition *)
+
+(** **** Initialize an environment
+
+  For each instant, local resource names that represent a reading interaction have their memory cells initialized as unused with a certain term. This function takes a reader environment [rs] and an environement [V] and produces an environment where all resource names in [rs] are initialized.
+*)
+Definition init_read_func (r : resource) (v : Λ) (V : 𝐕) := (⌈ r ⤆ ⩽ v … ⩾ ⌉ V)%re.
+
+Definition init_read (rs : t) (V : 𝐕) := fold init_read_func rs V.
+
+(** **** Halts 
+
+  In the functional transition proofs, we assume that all elements in the virtual resource environment [W] halts. Thus, we define this property here with [For_all].
+  An environment has the halting property if and only if each term in it halts. 
+*)
+Definition halts (k : lvl) := For_all (fun _ d => ET.halts k d).
+
+(** *** Property *)
+
+(** **** [extend] property *)
+ 
+Lemma extend_Empty_left_spec (rs rs' : t) :
+  Empty rs -> eq (extend rs rs') rs'.
+Proof.
+  intro HEmp; unfold extend.
+  apply Empty_eq_spec in HEmp.
+  rewrite fold_init; eauto.
+  - apply fold_identity.
+  - repeat red; intros; subst; now rewrite H1.
+Qed.
+
+Lemma extend_Empty_right_spec (rs rs' : t) :
+  Empty rs' -> eq (extend rs rs') rs.
+Proof. intro HEmp; unfold extend; now rewrite fold_Empty; eauto. Qed.
+
+Lemma extend_add_right_spec (r : resource) (v : Λ) (rs rs' : t) :
+  ~ (In r rs') -> eq (extend rs (add r v rs')) (add r v (extend rs rs')).
+Proof.
+  intro HnIn; unfold extend; rewrite fold_Add; eauto.
+  - reflexivity.
+  - intros k' k Heqk d' d Heqd c c' Heqc; subst; now rewrite Heqc.
+  - apply diamond_add.
+  - unfold ReadStock.Add; reflexivity.
+Qed.
+
+Lemma valid_extend_spec (k : lvl) (rs rs' : t) :
+  valid k rs -> valid k rs' -> valid k (extend rs rs').
+Proof.
+  revert rs; induction rs' using map_induction; intros rs Hvrs Hvrs'.
+  - rewrite extend_Empty_right_spec; auto.
+  - unfold ReadStock.Add in H0; rewrite H0 in *; clear H0.
+    rewrite extend_add_right_spec; auto.
+    apply valid_add_notin_spec in Hvrs' as [Hvx [Hve Hvrs'1]]; auto.
+    apply valid_add_spec; auto.
+Qed.
+
+
+(** **** [init_read] property *)
+
+#[export] Instance init_read_func_proper :
+ Proper (Logic.eq ==> Logic.eq ==> RE.eq ==> RE.eq) init_read_func.
+Proof.
+  intros k' k Heqk d' d Heqd V V' HeqV; subst; unfold init_read_func.
+  now rewrite HeqV.
+Qed.
+
+Lemma init_read_func_diamond : Diamond RE.eq init_read_func.
+Proof.
+  unfold init_read_func; intros k k' d d' rs rs1 rs' Hneq Heq Heq'.
+  rewrite <- Heq; rewrite <- Heq'.
+  now rewrite RE.add_add_2; auto.
+Qed.
+
+#[local] Hint Resolve init_read_func_proper init_read_func_diamond RE.Equal_equiv : core.
+
+Lemma init_read_Empty_spec (rs : t) (V : 𝐕) :
+  Empty rs -> RE.eq (init_read rs V) V.
+Proof.
+  intro Hemp; unfold init_read.
+  rewrite fold_Empty with (eqA := RE.eq); now auto.
+Qed.
+
+Lemma init_read_add_spec (r : resource) (v : Λ) (rs : t) (V : 𝐕) :
+  ~ (In r rs) ->
+  RE.eq (init_read (add r v rs) V) (⌈ r ⤆ (⩽ v … ⩾)⌉ (init_read rs V))%re. 
+Proof.
+  unfold init_read; intro HnIn.
+  rewrite fold_Add with (eqA := RE.eq); eauto.
+  - unfold init_read_func at 1; reflexivity.
+  - red; reflexivity.
+Qed.
+
+#[export] Instance init_read_proper : Proper (eq ==> RE.eq ==> RE.eq) init_read.
+Proof.
+  intros rs rs' Heqrs V V' HeqV; unfold init_read.
+  eapply fold_Proper with (eqA := RE.eq); now eauto.
+Qed.  
+
+Lemma init_read_find_spec (rs : t) (V : 𝐕) (r : resource) (v : 𝑣) :
+  ((init_read rs V)⌊r⌋)%re = Some v -> In r rs \/ V⌊r⌋%re = Some v.
+Proof.
+  revert r v; induction rs using map_induction; intros r v Hfi.
+  - rewrite init_read_Empty_spec in Hfi; auto.
+  - unfold ReadStock.Add in H0; rewrite H0 in *; clear H0.
+    rewrite init_read_add_spec in Hfi; auto.
+    rewrite RE.add_o in Hfi; destruct (Resource.eq_dec x r) as [| Hneq]; subst.
+    -- now rewrite add_in_iff; repeat left.
+    -- rewrite add_in_iff.
+       apply IHrs1 in Hfi as [HIn | Hfi]; auto.
+Qed. 
+
+Lemma init_read_in_iff  (rs : t) (V : 𝐕) (r : resource) :
+  (r ∈ (init_read rs V))%re <-> In r rs \/ (r ∈ V)%re.
+Proof.
+  revert r; induction rs using map_induction; intro r; split.
+  - rewrite init_read_Empty_spec; auto.
+  - intros [HIn | HIn].
+    -- destruct HIn as [v HM].
+       exfalso; now apply (H r v).
+    -- rewrite init_read_Empty_spec; auto.
+  - intro HIn.
+    unfold ReadStock.Add in H0; rewrite H0 in *; clear H0.
+    rewrite init_read_add_spec in HIn; auto.
+    rewrite add_in_iff.
+    apply RE.add_in_iff in HIn as [| HIn]; subst; auto.
+    apply IHrs1 in HIn as [HIn | HIn]; auto.
+  - unfold ReadStock.Add in H0; rewrite H0 in *; clear H0.
+    rewrite add_in_iff.
+    rewrite init_read_add_spec; auto.
+    rewrite RE.add_in_iff.
+    intros [[Heq | HIn] | HIn]; subst; auto; 
+    right; rewrite IHrs1; auto.
+Qed. 
+
+Lemma init_read_unused (rs : t) (V : 𝐕) (r : resource) :
+  In r rs -> REnvironment.unused r (init_read rs V).
+Proof.
+  revert r; induction rs using map_induction; intros r HIn.
+  - exfalso; destruct HIn as [v HM]; now apply (H r v).
+  - unfold ReadStock.Add in H0; rewrite H0 in *; clear H0.
+    rewrite init_read_add_spec; auto; 
+    apply add_in_iff in HIn as [| HIn]; subst.
+    -- apply RE.unused_add_eq_spec; now red.
+    -- assert (Hneq : r <> x) by (intro; subst; contradiction).
+       apply RE.unused_add_neq_spec; auto.
+Qed.
+
+(* Lemma init_read_Forall_unused : forall rsk V,
+  REnvironment.For_all (fun _ v => Cell.unused v) V ->
+  REnvironment.For_all (fun _ v => Cell.unused v) (init_read rsk V).
+Proof.
+  unfold REnvironment.For_all in *; intros.
+  apply init_read_find_spec in H0 as H0'; destruct H0'; auto.
+  - eapply init_read_unused in H1; eauto.
+    destruct H1; rewrite H0 in H1; inversion H1. now simpl.
+  - eapply H; eauto.
+Qed. *)
+
+
+(** **** [halts] property *)
+
+Lemma halts_union_spec (k : lvl) (rs rs': t) :
+  halts k rs /\ halts k rs' -> halts k (extend rs rs').
+Proof.
+  unfold halts; intros [HFa HFa'] r v Hfi.
+  apply find_2 in Hfi. 
+  apply extend_mapsto_iff in Hfi as [HM | [HM _]]; apply find_1 in HM.
+  - now apply (HFa' r).
+  - now apply (HFa r).
+Qed.
+
+Lemma halts_add_spec (k : lvl) (r : resource) (v : Λ) (rs : t) :
+  (ET.halts k v) /\ halts k rs -> halts k (add r v rs).
+Proof.
+  intros [Hltv Hlts] r' v' Hfi.
+  rewrite add_o in Hfi; destruct (Resource.eq_dec r r') as [| Hneq]; subst.
+  - inversion Hfi; subst; auto.
+  - apply Hlts in Hfi; auto.
+Qed.
+
+Lemma halts_add_iff (k : lvl) (r : resource) (v : Λ) (rs : t) :
+  ~ (In r rs) -> 
+  halts k (add r v rs) <-> (ET.halts k v) /\ halts k rs.
+Proof.
+  intros HIn; split.
+  - unfold halts; intro HFa.
+    apply For_all_add_notin_spec in HFa; auto.
+  - apply halts_add_spec.
+Qed.
+
+Lemma halts_weakening (m n : lvl) (rs : t) : 
+  m <= n -> halts m rs -> halts n (shift m (n - m) rs).
+Proof.
+  intros Hle Hlt r v Hfi. 
+  apply shift_find_e_spec_1 in Hfi as HI.
+  destruct HI as [[r' Heqr'] [v' Heqv']]; subst.
+  rewrite <- shift_find_iff in Hfi. 
+  apply ET.halts_weakening; auto; apply Hlt in Hfi; now simpl in *.
+Qed.
+
+Lemma halts_weakening_1 (m n : lvl) (rs : t) : 
+  halts m rs -> halts (m + n) (shift m n rs).
+Proof.
+  intro Hlt; replace n with ((m + n) - m) at 2 by lia.
+  apply halts_weakening; auto; lia.
+Qed.
+
+Lemma halts_init_read (k : lvl) (rs : t) (V : 𝐕) :
+  halts k rs -> RE.halts k V -> RE.halts k (init_read rs V).
+Proof.
+  induction rs using map_induction; intros Hltrs HltV.
+  - now rewrite init_read_Empty_spec.
+  - unfold ReadStock.Add in H0; rewrite H0 in *; clear H0.
+    rewrite init_read_add_spec; auto.
+    apply RE.halts_add_spec; simpl.
+    apply halts_add_iff in Hltrs as [Hkte Htlrs1]; auto. 
+Qed.
+
+(** **** Morphism *)
+
+#[export] Instance in_readstock : Proper (Logic.eq ==> eq ==> iff) In.
+Proof. intros k' k Heqk rs rs' Heqrs; subst; now rewrite Heqrs. Qed.
+
+#[export] Instance Add_readstock : 
+  Proper (Resource.eq ==> Term.eq ==> eq ==> eq ==> iff) (@ReadStock.Add Term.t).
+Proof.
+  intros k' k Heqk d d' Heqd rs rs' Heqrs rs1 rs1' Heqrs1; unfold ReadStock.Add.
+  now rewrite Heqk, Heqd, Heqrs, Heqrs1. 
+Qed.
+
+#[export] Instance halts_readstock : Proper (Logic.eq ==> eq ==> iff) halts. 
+Proof. unfold halts; intros m n Heqm rs rs' Heqrs; subst; now rewrite Heqrs. Qed.
+
+End ReadStock.
+
+(** ---- *)
+
+(** ** Notation - Virtual Resource Environment - Reader *)
+
+Module ReadStockNotations.
+
+(** *** Scope *)
+Declare Scope rstock_scope.
+Delimit Scope rstock_scope with rk.
+
+(** *** Notation *)
+Definition 𝐖ᵣ := ReadStock.t.
+
+Notation "V '⁺'" := (ReadStock.Ext.new_key V) (at level 16) : rstock_scope.
+Notation "∅" := ReadStock.Raw.empty (at level 0, no associativity) : rstock_scope. 
+Notation "r '∉' Re" := (~ (ReadStock.Raw.In r Re)) (at level 75, no associativity) : rstock_scope. 
+Notation "'isEmpty(' Re ')'" := (ReadStock.Empty Re) (at level 20, no associativity) : rstock_scope. 
+Notation "'Add'" := (ReadStock.Add) (at level 20, no associativity) : rstock_scope. 
+Notation "R '⌊' x '⌋'"  := (ReadStock.Raw.find x R) (at level 15, x constr) : rstock_scope.
+Notation "'max(' R ')'"  := (ReadStock.Ext.max_key R) (at level 15) : rstock_scope.
+Notation "⌈ x ⤆ v '⌉' R" := (ReadStock.Raw.add x v R) 
+                             (at level 15, x constr, v constr) : rstock_scope.
+Notation "'[⧐' lb '–' k ']' t" := (ReadStock.shift lb k t) 
+                                   (at level 65, right associativity) : rstock_scope.
+
+Infix "⊆" := ReadStock.Submap (at level 60, no associativity) : rstock_scope. 
+Infix "∈" := ReadStock.Raw.In (at level 60, no associativity) : rstock_scope. 
+Infix "=" := ReadStock.eq : rstock_scope.
+Infix "∪" := ReadStock.extend : rstock_scope.
+Infix "⊩" := ReadStock.valid (at level 20, no associativity) : rstock_scope.
+
+(** *** Morphism *)
+
+Import ReadStock.
+
+#[export] Instance max_rk : Proper (eq ==> Logic.eq) (Ext.max_key) := Ext.max_key_eq.
+#[export] Instance new_rk : Proper (eq ==> Logic.eq) (Ext.new_key) := Ext.new_key_eq.
+#[export] Instance in_rk : Proper (Logic.eq ==> ReadStock.eq ==> iff) (ReadStock.Raw.In) := _.
+#[export] Instance find_rk : Proper (Logic.eq ==> eq ==> Logic.eq) (Raw.find) := _.
+#[export] Instance Empty_rk : Proper (ReadStock.eq ==> iff) (ReadStock.Empty) := _.
+#[export] Instance Add_rk : 
+  Proper (Resource.eq ==> Term.eq ==> eq ==> eq ==> iff) (@ReadStock.Add Term.t) := _.
+#[export] Instance add_rk : 
+  Proper (Resource.eq ==> Term.eq ==> eq ==> eq) (@Raw.add Term.t) := _.
+#[export] Instance Submap_rk : Proper (eq ==> eq ==> iff) Submap := _.
+#[export] Instance Submap_rk_po : PreOrder ReadStock.Submap := Submap_po.
+#[export] Instance valid_rk : Proper (Logic.eq ==> ReadStock.eq ==> iff) ReadStock.valid := _.
+#[export] Instance shift_rk : Proper (Logic.eq ==> Logic.eq ==> eq ==> eq) shift := _.
+#[export] Instance halts_rk: Proper (Logic.eq ==> ReadStock.eq ==> iff) ReadStock.halts := _.
+
+End ReadStockNotations.
